Some work on LR.

Stlc/SpecEvaluation.v
@@ -151,3 +151,7 @@ Proof.
   induction C; cbn in *; intuition.
 Qed.
 
+Inductive evaln (t : Tm) : Tm → nat → Prop :=
+| evaln_zero : evaln t t 0
+| evaln_step : forall t' t'' n, t --> t' → evaln t' t'' n → evaln t t'' (S n).
+
